Define equivalence relation

reform/translation.v
@@ -6,4 +6,94 @@ Require Import Lt Le Gt.
 Require Sorts PTS PTS_Ext.
 Module S := PTS_Ext.
 Module T := PTS.
-Import T Sorts.withoutProp.
+Import T Sorts Sorts.withoutProp.
+
+(* We first would like to express an equivalence between terms that can either
+   be in S or in T. If we only look at the terms, then S is included in T. *)
+Fixpoint ι (t : S.Term) : Term :=
+  match t with
+  | S.Var x => #x
+  | S.Sort s => !s
+  | S.Π A B => Π (ι A) (ι B)
+  | S.λ A t => λ (ι A) (ι t)
+  | S.App t u => (ι t) · (ι u)
+  | S.Eq A u v => Eq (ι A) (ι u) (ι v)
+  | S.refle t => refle (ι t)
+  | S.J A P M1 N M2 p => J (ι A) (ι P) (ι M1) (ι N) (ι M2) (ι p)
+  end.
+
+(* We also need to define the notion of transport inside T. *)
+(* Reserved Notation "p ⋆ t" (at level 30). *)
+Definition transport (s : Sorts) (A B p : Term) : Term :=
+  λ A (J !s #0 (A ↑) #0 (B ↑) (p ↑)).
+(* Notation "p ⋆ a" := ((transport ? ? ? p) · a) *)
+
+Lemma subst0 : forall t n, t ↑ 0 # n = t.
+Admitted.
+
+Lemma transport_typ :
+  forall Γ s A B p,
+    Γ ⊢ A : !s -> Γ ⊢ B : !s ->
+    Γ ⊢ p : Eq !s A B ->
+    Γ ⊢ transport s A B p : A ⇒ B.
+Proof.
+  intros Γ s A B p hA hB hp.
+  induction s. eapply cλ.
+  - exact (Rel0 n n).
+  - exact hA.
+  - admit. (* Weakening *)
+  - cut (
+      A :: Γ ⊢ J !(U n) #0 (A ↑) #0 (B ↑) (p ↑) : (#0)[← B ↑]
+    ).
+    + simpl. rewrite subst0. auto.
+    + eapply cJ.
+      * { apply cVar.
+          - eapply wf_cons. apply cSort.
+            + eapply wf_cons. exact hA.
+            + apply (Ax0 n (S n)). auto.
+          - exists ! (U n) ; split.
+              + simpl. auto.
+              + apply item_hd.
+        }
+      * simpl. rewrite subst0.
+        { apply cVar.
+          - eapply wf_cons. exact hA.
+          - exists A ; split ; auto.
+        }
+      * admit. (* Weakening *)
+Admitted.
+
+(* We can now express our relation on T terms. *)
+Reserved Notation "t ~ u" (at level 80, no associativity).
+Reserved Notation "t ≃ u @ E" (at level 80, no associativity).
+
+(* For the purpose of the proof we define an extension of the relation first. *)
+Inductive equiv (E : list (Vars * Vars)) : Term -> Term -> Prop :=
+| EquivGen : forall (x y : Vars), In (x,y) E -> #x ≃ #y @ E
+| EquivVar : forall (x : Vars), #x ≃ #x @ E
+| EquivTL  : forall t1 t2 s A B p,
+               t1 ≃ t2 @ E -> (transport s A B p) · t1 ≃ t2 @ E
+| EquivTR  : forall t1 t2 s A B p,
+               t1 ≃ t2 @ E -> t1 ≃ (transport s A B p) · t2 @ E
+| EquivApp : forall t1 t2 u1 u2, t1 ≃ t2 @ E -> u1 ≃ u2 @ E -> t1 · u1 ≃ t2 · u2 @ E
+| Equivλ   : forall A1 A2 t1 t2, A1 ≃ A2 @ E -> t1 ≃ t2 @ E -> λ A1 t1 ≃ λ A2 t2 @ E
+| EquivΠ   : forall A1 A2 B1 B2, A1 ≃ A2 @ E -> B1 ≃ B2 @ E -> Π A1 B1 ≃ Π A2 B2 @ E
+| EquivEq  : forall A1 A2 u1 u2 v1 v2,
+               A1 ≃ A2 @ E -> u1 ≃ u2 @ E -> v1 ≃ v2 @ E ->
+               Eq A1 u1 v1 ≃ Eq A2 u2 v2 @ E
+| EquivRfl : forall t1 t2, t1 ≃ t2 @ E -> refle t1 ≃ refle t2 @ E
+| EquivJ   : forall A1 A2 P1 P2 u1 u2 t1 t2 v1 v2 p1 p2,
+               A1 ≃ A2 @ E -> P1 ≃ P2 @ E -> u1 ≃ u2 @ E -> t1 ≃ t2 @ E ->
+               v1 ≃ v2 @ E -> p1 ≃ p2 @ E ->
+               J A1 P1 u1 t1 v1 p1 ≃ J A2 P2 u2 t2 v2 p2 @ E
+where "t ≃ u @ E" := (equiv E t u).
+
+Notation "t ~ u" := (t ≃ u @ nil).
+
+(* Now let's see how such terms relate. *)
+(* Lemma equiv_equal : *)
+(*   forall Γ t1 t2 T1 T2, *)
+(*     Γ ⊢ t1 : T1 -> Γ ⊢ t2 : T2 -> t1 ~ t2 -> *)
+(*     exists p, Γ ⊢ p : (* We need Σ-types... *) *)
+
+
